src/study/Nemonuri.Study.CSharpSyntaxRewriter2.Modifier2/Nemonuri.StratifiedNodes.Children.fst
@@ -7,8 +7,23 @@ module N = Nemonuri.StratifiedNodes.Nodes
 
 //---|
 
+//--- theory members ---
 let is_child #t (parent_node:N.node t) (node:N.node t) 
-  : Tot (b:bool{if b then (N.get_level node) < (N.get_level parent_node) else true})
+  : Pure bool (requires True) (ensures fun _ -> N.node_level_is_greater_than_levels_of_nodes_in_children t)
+    //Tot (b:bool{N.node_level_is_greater_than_levels_of_nodes_in_children t}) 
+    //if b then (N.get_level node) < (N.get_level parent_node) else true
   =
+  N.lemma_node_level_is_greater_than_levels_of_nodes_in_children t;
   L.contains node (N.get_children parent_node)
 
+(*
+  let result = (L.contains node (N.get_children parent_node)) in
+  if result then
+    (
+      N.lemma_node_level_is_greater_than_level_of_node_in_children parent_node node;
+      true
+    )
+  else
+    false
+*)
+//---|
